policy_proof/coq/query.v
@@ -5,28 +5,55 @@ Require Import types.
 Require Import relation.
 Require Import formula.
 Require Import data_model.
+Require Import ordering.
+Require Import finite_bags.
 
-Definition project_list : Set := list simple_atomic_expression%type.
-
-Fixpoint bounded_list (proj: project_list) (ty: Tuple.tuple_type) : Prop :=
-  match proj with
-    | nil => True
-    | h :: t => match h with
-                  | simple_atomic_expression_column n => n < List.length ty
-                  | _ => True
-                end /\ bounded_list t ty
+Fixpoint schema_to_anf (s: schema): list nat :=
+  match s with
+    | nil => nil
+    | cons t ty' => cons 0 (List.map S (schema_to_anf ty'))
   end.
 
-Inductive Query: schema -> Set :=
-  | query_empty: forall s, Query s
-  | query_relation: forall s, relation s -> Query s
-  | query_union: forall s, Query s -> Query s -> Query s
-  | query_join: forall s1 s2, Query s1 -> Query s2 -> Query (s1 ++ s2)
-  | query_project:
-      forall s (proj: project_list) (bounded: bounded_list proj (schema_denote s)),
-        Query s -> Query s
-  | query_select:
-    forall s (where_exp: simple_formula), Query s -> Query s
-  (* TODO: Design `groupby`. *)
-  | query_grouby_agg: forall s, Query s -> Query s
-  .
+Inductive project_list: Set :=
+  | project_star: project_list
+  | project s: list (forall bt, agg_expression s bt) -> project_list
+.
+
+Definition groupby_list := (list nat)%type.
+Definition agg_list s := (list (forall bt, agg_expression s bt))%type.
+
+Definition context: Set := list (nat * schema)%type.
+Fixpoint env (ctx: context): Set :=
+  match ctx with
+    | nil => unit
+    | (_, s) :: ctx' => relation s * env ctx'
+  end%type.
+
+(* TODO: we also need to reason about how schema (type) is changed in the course of operators. *)
+Inductive Operator: schema -> Set :=
+  | operator_empty: forall s, Operator s
+  | operator_relation: forall s, nat -> Operator s
+  | operator_union: forall s, Operator s -> Operator s -> Operator s
+  | operator_join: forall s1 s2, Operator s1 -> Operator s2 -> Operator (s1 ++ s2)
+  | operator_project: forall s, project_list -> Operator s -> Operator s
+  | operator_select: forall s, formula s -> Operator s -> Operator s
+  | operator_grouby_having: forall s, groupby_list -> agg_list s -> formula s -> Operator s -> Operator s
+.
+
+Definition config (ctx: context) := (Policy.context * Configuration.privacy * Operator ((snd (List.hd (0, nil) ctx))) * env ctx)%type.
+
+(**  
+  [eval] is a Fixpoint in Coq, which means it is a recursive function. It is used to evaluate a
+  query on a given configuration and schema.
+
+  @param c   A configuration of type [config s]. This configuration is a tuple containing a Policy
+             context, an environment, a privacy setting, an Operator, and a tuple type.
+
+  @return    The result of the evaluation of the query on the given configuration.
+*)
+Fixpoint eval (ctx: context) (c: config ctx): option (config ctx) :=
+  match get_operator c with
+  | operator_empty => None
+  (* TODO: IMPLEMENT THIS. *)
+  | _ => None 
+  end.
