policy_proof/coq/relation.v
@@ -7,8 +7,6 @@ Require Import ordering.
 Require Import finite_bags.
 Require Import types.
 
-Definition schema_denote (s: schema): Tuple.tuple_type := List.map (fun x => (fst x)) s.
-
 (** 
   [relation_np] is a function that takes a tuple type [ty] as an argument and returns a finite bag (fbag) of tuples of type [ty]. 
   This function is used to define a relation in the context of a database or a similar data structure where relations are represented as collections of tuples.
@@ -16,7 +14,7 @@ Definition schema_denote (s: schema): Tuple.tuple_type := List.map (fun x => (fs
   @param s   The schema of the relation.
   @return    A finite bag (fbag) of tuples of type [ty].
 *)
-Definition relation_np (s: schema) := fbag (Tuple.tuple_np (schema_denote s)).
+Definition relation_np (s: schema) := fbag (Tuple.tuple_np s).
 
 (** 
   [relation] is a function that takes a tuple type [ty] as an argument and returns a finite bag (fbag) of tuples of type [ty]. 
@@ -25,7 +23,7 @@ Definition relation_np (s: schema) := fbag (Tuple.tuple_np (schema_denote s)).
   @param s   The schema of the relation.
   @return    A finite bag (fbag) of tuples of type [ty].
 *)
-Definition relation (s: schema) := fbag (Tuple.tuple (schema_denote s)).
+Definition relation (s: schema) := fbag (Tuple.tuple s).
 
 (**
   [inject_tuple_id_relation] is a function that takes a tuple type [ty], a relation [r] of type [relation_np ty] and an id [id] as arguments and returns a relation of type [relation ty].
@@ -43,7 +41,6 @@ Fixpoint inject_tuple_id_relation
   match r with
   | nil => nil
   | cons t r' =>
-    let ty := (schema_denote s) in
-      cons (Tuple.inject_tuple_id ty t id) (inject_tuple_id_relation s r' (id + List.length ty))
+  cons (Tuple.inject_tuple_id s t id)
+       (inject_tuple_id_relation s r' (id + List.length s))
   end.
-
